AwsCryptographicMaterialProviders/dafny/AwsCryptographyKeyStore/test/Fixtures.dfy
@@ -102,6 +102,7 @@ module Fixtures {
   const KmsSrkConfigWest : Types.KMSConfiguration := Types.KMSConfiguration.kmsKeyArn(MrkArnWest)
   const KmsMrkConfigAP : Types.KMSConfiguration := Types.KMSConfiguration.kmsMRKeyArn(MrkArnAP)
   const KmsMrkEC : Types.EncryptionContext := map[UTF8.EncodeAscii("abc") := UTF8.EncodeAscii("123")]
+  const RobbieEC : Types.EncryptionContext := map[UTF8.EncodeAscii("Robbie") := UTF8.EncodeAscii("is a dog.")]
   const EastBranchKey : string := "MyEastBranch2"
   const EastBranchKeyIdActiveVersion : string := "6f22825b-bd56-4434-83e2-2782e2160172"
   const EastBranchKeyBranchKeyIdActiveVersionUtf8Bytes: seq<uint8> := [
