AwsCryptographicMaterialProviders/dafny/AwsCryptographyKeyStoreAdmin/test/TestAdminCreateKeys.dfy
@@ -4,8 +4,7 @@
 include "../src/Index.dfy"
 include "../../AwsCryptographyKeyStore/test/CleanupItems.dfy"
 include "../../AwsCryptographyKeyStore/test/Fixtures.dfy"
-include "../../AwsCryptographyKeyStore/test/TestGetKeys.dfy"
-include "../../AwsCryptographyKeyStore/Model/AwsCryptographyKeyStoreTypes.dfy"
+include "../../AwsCryptographyKeyStore/test/BranchKeyValidators.dfy"
 include "AdminFixtures.dfy"
 
 module {:options "/functionSyntax:4" } TestAdminCreateKeys {
@@ -22,38 +21,118 @@ module {:options "/functionSyntax:4" } TestAdminCreateKeys {
   import UUID
   import CleanupItems
   import AdminFixtures
-  import TestGetKeys
+  import BranchKeyValidators
 
-  // method {:test} TestCreateBranchAndBeaconKeys()
-  // {
-  //   var ddbClient :- expect Fixtures.ProvideDDBClient();
-  //   var kmsClient :- expect Fixtures.ProvideKMSClient();
-  //   var storage :- expect Fixtures.DefaultStorage(ddbClient?:=Some(ddbClient));
-  //   var keyStore :- expect Fixtures.DefaultKeyStore(ddbClient?:=Some(ddbClient), kmsClient?:=Some(kmsClient));
-  //   var strategy :- expect AdminFixtures.DefaultKeyManagerStrategy(kmsClient?:=Some(kmsClient));
-  //   var underTest :- expect AdminFixtures.DefaultAdmin(ddbClient?:=Some(ddbClient));
+  // TODO-HV-2-FOLLOW : TestCreateSRKForHV1, TestCreateForHV1NoBKID, TestCreateForHV1BbkidNoECFails
 
-  //   var input := Types.CreateKeyInput(
-  //     Identifier := None,
-  //     EncryptionContext := None,
-  //     KmsArn := Types.KmsSymmetricKeyArn.KmsKeyArn(keyArn),
-  //     Strategy := Some(strategy)
-  //   );
-  //   var identifier? :- expect underTest.CreateKey(input);
-  //   var identifier := identifier?.Identifier;
-  //   expect identifier?.HierarchyVersion == KeyStoreTypes.HierarchyVersion.v1,
-  //     "KeyStoreAdmin should create branch key with `hierarchy-version-1` when no `HierarchyVersion` provided";
+  const happyCaseId := "test-happy-case-admin-create-key-hv-1"
+  method {:test} TestCreateMRKForHV1()
+  {
+    var ddbClient :- expect Fixtures.ProvideDDBClient();
+    var kmsClient :- expect Fixtures.ProvideKMSClient();
+    var storage :- expect Fixtures.DefaultStorage(ddbClient?:=Some(ddbClient));
+    var keyStore :- expect Fixtures.DefaultKeyStore(ddbClient?:=Some(ddbClient), kmsClient?:=Some(kmsClient));
+    var strategy :- expect AdminFixtures.DefaultKeyManagerStrategy(kmsClient?:=Some(kmsClient));
+    var underTest :- expect AdminFixtures.DefaultAdmin(ddbClient?:=Some(ddbClient));
+    var keyStoreEast :- expect KeyStoreFromKMSConfig(
+      kmsConfig := KmsMrkConfigEast,
+      ddbClient? := Some(ddbClient)
+    );
+    var uuid :- expect UUID.GenerateUUID();
+    var bkid := happyCaseId + "-west-mrk-" + uuid;
+    // Create an HV-1 BK with a West MRK by calling us-west-2
+    var bk :- expect underTest.CreateKey(
+      Types.CreateKeyInput(
+        Identifier := Some(bkid),
+        EncryptionContext := Some(KmsMrkEC),
+        KmsArn := Types.KmsSymmetricKeyArn.KmsMRKeyArn(MrkArnWest),
+        // us-west-2 b/c CI region is us-west-2 and KMS Client is created
+        Strategy := Some(strategy)
+      ));
+    expect bk.Identifier == bkid;
+    // Validate an HV-1 BK with a West MRK by calling us-east-1
+    BranchKeyValidators.VerifyGetKeys(bkid, keyStoreEast, storage,
+                                      encryptionContext := KmsMrkEC);
+    var keyStoreWest :- expect KeyStoreFromKMSConfig(
+      // Passing in KmsMrkConfigWest causes the KMS Client to be created for us-west-2
+      // bk's KMS-ARN is replicated to us-west-2
+      kmsConfig := KmsMrkConfigWest,
+      ddbClient? := Some(ddbClient)
+    );
+    // Validate an HV-1 BK with a West MRK by calling us-west-2
+    BranchKeyValidators.VerifyGetKeys(bkid, keyStoreWest, storage,
+                                      encryptionContext := KmsMrkEC);
+    var _ := CleanupItems.DeleteBranchKey(Identifier:=bkid, ddbClient:=ddbClient);
+  }
 
-  //   // Get branch key items from storage
-  //   TestGetKeys.VerifyGetKeys(
-  //     identifier := identifier,
-  //     keyStore := keyStore,
-  //     storage := storage
-  //   );
+  const happyCaseIdHV2 := "test-happy-case-admin-create-key-hv-2"
+  method {:test} TestCreateMRKForHV2()
+  {
+    var ddbClient :- expect Fixtures.ProvideDDBClient();
+    var kmsClient :- expect Fixtures.ProvideKMSClient();
+    var storage :- expect Fixtures.DefaultStorage(ddbClient?:=Some(ddbClient));
+    var strategy :- expect AdminFixtures.SimpleKeyManagerStrategy(kmsClient?:=Some(kmsClient));
+    var underTest :- expect AdminFixtures.DefaultAdmin(ddbClient?:=Some(ddbClient));
+    var keyStoreEast :- expect KeyStoreFromKMSConfig(
+      kmsConfig := KmsMrkConfigEast,
+      ddbClient? := Some(ddbClient)
+    );
+    var uuid :- expect UUID.GenerateUUID();
+    var bkid := happyCaseIdHV2 + "-west-mrk-" + uuid;
+    // Create an HV-2 BK with a West MRK by calling us-west-2
+    var bk :- expect underTest.CreateKey(
+      Types.CreateKeyInput(
+        Identifier := Some(bkid),
+        EncryptionContext := Some(RobbieEC),
+        KmsArn := Types.KmsSymmetricKeyArn.KmsMRKeyArn(MrkArnWest),
+        // us-west-2 b/c CI region is us-west-2 and KMS Client is created
+        Strategy := Some(strategy),
+        HierarchyVersion := Some(KeyStoreTypes.HierarchyVersion.v2)
+      ));
+    expect bk.Identifier == bkid;
+    // Validate an HV-2 BK with a West MRK by calling us-east-1
+    BranchKeyValidators.VerifyGetKeys(bkid, keyStoreEast, storage,
+                                      encryptionContext := RobbieEC,
+                                      hierarchyVersion := KeyStoreTypes.HierarchyVersion.v2);
+    var keyStoreWest :- expect KeyStoreFromKMSConfig(
+      // Passing in KmsMrkConfigWest causes the KMS Client to be created for us-west-2
+      // bk's KMS-ARN is replicated to us-west-2
+      kmsConfig := KmsMrkConfigWest,
+      ddbClient? := Some(ddbClient)
+    );
+    // Validate an HV-2 BK with a West MRK by calling us-west-2
+    BranchKeyValidators.VerifyGetKeys(bkid, keyStoreWest, storage,
+                                      encryptionContext := RobbieEC,
+                                      hierarchyVersion := KeyStoreTypes.HierarchyVersion.v2);
+    var _ := CleanupItems.DeleteBranchKey(Identifier:=bkid, ddbClient:=ddbClient);
+  }
 
-  //   // Since this process uses a read DDB table,
-  //   // the number of records will forever increase.
-  //   // To avoid this, remove the items.
-  //   var _ := CleanupItems.DeleteBranchKey(Identifier:=identifier, ddbClient:=ddbClient);
-  // }
+  method {:test} TestCreateSRKForHV2()
+  {
+    var ddbClient :- expect Fixtures.ProvideDDBClient();
+    var kmsClient :- expect Fixtures.ProvideKMSClient();
+    var storage :- expect Fixtures.DefaultStorage(ddbClient?:=Some(ddbClient));
+    var keyStore :- expect Fixtures.DefaultKeyStore(ddbClient?:=Some(ddbClient), kmsClient?:=Some(kmsClient));
+    var strategy :- expect AdminFixtures.SimpleKeyManagerStrategy(kmsClient?:=Some(kmsClient));
+    var underTest :- expect AdminFixtures.DefaultAdmin(ddbClient?:=Some(ddbClient));
+    var uuid :- expect UUID.GenerateUUID();
+    var bkid := happyCaseIdHV2 + "-west-srk-" + uuid;
+    // Create an HV-2 BK with a West MRK by calling us-west-2
+    var bk :- expect underTest.CreateKey(
+      Types.CreateKeyInput(
+        Identifier := Some(bkid),
+        EncryptionContext := Some(RobbieEC),
+        KmsArn := Types.KmsSymmetricKeyArn.KmsKeyArn(keyArn),
+        // us-west-2 b/c CI region is us-west-2 and KMS Client is created
+        Strategy := Some(strategy),
+        HierarchyVersion := Some(KeyStoreTypes.HierarchyVersion.v2)
+      ));
+    expect bk.Identifier == bkid;
+    // Validate an HV-2 BK with a West MRK by calling us-east-1
+    BranchKeyValidators.VerifyGetKeys(bkid, keyStore, storage,
+                                      encryptionContext := RobbieEC,
+                                      hierarchyVersion := KeyStoreTypes.HierarchyVersion.v2);
+    var _ := CleanupItems.DeleteBranchKey(Identifier:=bkid, ddbClient:=ddbClient);
+  }
+
 }
